\section*{Problem 3 Solution}

\begin{enumerate}[a)]

\item 

\begin{align*}
\frac{dy}{dx}	&= -3y \\
\frac{dy}{y} 	& = -3\,dx \\
\int\frac{dy}{y}&= -3 \int \,dx \\
\ln y			&= -3 x + C \\
y				&= e^{-3x + C} \\
\end{align*}
$$\boxed{y = Ce^{-3x}}$$

\item 

Solve the second order differential equation
$$ \frac{d^2 y}{dx^2} - A^2y = B $$
For the homogeneous equation, $\frac{d^2 y}{dx^2} - A^2y = 0$, try $y_c = X_1 e^{Ax} + X_2 e^{-Ax}$ as the complementary solution ($X_1$ and $X_2$ are constants). Then
$$ \frac{d^2 y}{dx^2} = X_1 A^2 e^{Ax} + X_2 A^2 e^{-Ax} $$
and
$$ (X_1 A^2 e^{Ax} + X_2 A^2 e^{-Ax}) - A^2(X_1 e^{Ax} + X_2 e^{-Ax}) = 0 $$
$$ A^2 (X_1 e^{Ax} + X_2 e^{-Ax}) - A^2 (X_1 e^{Ax} + X_2 e^{-Ax}) = 0 $$

This is \underline{true}.

For the inhomogeneous equation, $\frac{d^2 y}{dx^2} - A^2y = B$, $y_P = -B/A^2$ is the only particular solution satisfying the equation. The general solution is the sum of the complementary and particular solutions, $y = y_c + y_p$. 
$$ y = X_1 e^{Ax} + X_2 e^{-Ax} - \frac{B}{A^2} $$
Now we can solve for $X_1$ and $X_2$. 
$$ y(\frac{1}{A}) = X_1 e^{A(\frac{1}{A})} + X_2 e^{-A(\frac{1}{A})} - \frac{B}{A^2} = 0 $$
and
$$ y(-\frac{1}{A}) = X_1 e^{A(-\frac{1}{A})} + X_2 e^{A(\frac{1}{A})} - \frac{B}{A^2} = 0 $$
We can note that in these two equations, $X_1$ and $X_2$ can be interchanged freely, and so must be equal. We will say, $X_1 = X_2 = X$. Then, we have
$$ 0 = X e^{A(-\frac{1}{A})} + X e^{A(\frac{1}{A})} - \frac{B}{A^2} $$
$$ 0 = X (e^{-1} + e^{1}) - \frac{B}{A^2} $$
$$ X = \frac{B}{A^2(\frac{1}{e} + e)} $$
The we plug this $X$ into the final solution, which gives
$$ y = \frac{B}{A^2(\frac{1}{e} + e)} (e^{Ax} + e^{-Ax}) - \frac{B}{A^2} $$
\end{enumerate}
Note that $e^{Ax} + e^{-Ax}$ is similar in form to $\cosh(Ax)$ which we could have also used to solve this problem.

